@prefix pt: <http://parliament.uk/ontologies/time-period/> . 
@prefix xsd: <http://www.w3.org/2001/XMLSchema#> . 
@prefix rdf: <http://www.w3.org/1999/02/22-rdf-syntax-ns#> .
@prefix dcterms: <http://purl.org/dc/terms/> .
@prefix owl:     <http://www.w3.org/2002/07/owl#> .
@prefix rdfs:    <http://www.w3.org/2000/01/rdf-schema#> .

<http://parliament.uk/ontologies/time-point/> 
    rdf:type owl:Ontology ;
    dcterms:title "Time period ontology"@en ;
    dcterms:created "09/03/2017"^^xsd:date ;
	dcterms:rights "Open Parliament Licence v3.0"@en ;
    dcterms:description "Ontology to describe high level time periods for UK Parliament"@en .


#######  Classes #####

pt:Agent rdf:type owl:Class ;
	rdfs:label "Agent"@en ;
	rdfs:comment "An agent. The superset of all people and all groups of people."@en ;
	rdf:isDefinedBy <http://parliament.uk/ontologies/time-period/> .

pt:Event rdf:type owl:Class ;
	rdfs:label "Event"@en ;
	rdfs:comment "A discrete event involving agents, locations and / or outputs. Events frequently initiate changes between time periods. Examples might be: State Opening, coronation, abdication, general election, prorogation, dissolution, recall."@en ;
	rdf:isDefinedBy <http://parliament.uk/ontologies/time-period/> .

pt:TimePeriod rdf:type owl:Class ;
	rdfs:label "TimePeriod"@en ;
	rdfs:comment "An identifiable and named period of time."@en ;
	rdf:isDefinedBy <http://parliament.uk/ontologies/time-period/> .

pt:Party rdf:type owl:Class ;
	rdfs:label "Party"@en ;
	rdfs:comment "An organised political group."@en ;
	rdf:isDefinedBy <http://parliament.uk/ontologies/time-period/> .

pt:GovernmentAdministrationPeriod rdf:type owl:Class ;
	rdfs:subClassOf pt:TimePeriod ;
	rdfs:label "GovernmentAdministrationPeriod"@en ;
	rdfs:comment "A period of a single government under a single prime minister bounded by parliaments / general elections. e.g. Thatcher administration 1979-1983, Thatcher administration 1983-1987, Thatcher administration 1987-1990."@en ;
	rdf:isDefinedBy <http://parliament.uk/ontologies/time-period/> .

pt:PremiershipPeriod rdf:type owl:Class ;
	rdfs:subClassOf pt:TimePeriod ;
	rdfs:label "PremiershipPeriod"@en ;
	rdfs:comment "A period of government under a single prime minister not bounded by parliaments / general elections. e.g. Thatcher administration 1979-1990."@en ;
	rdf:isDefinedBy <http://parliament.uk/ontologies/time-period/> .

pt:Reign rdf:type owl:Class ;
	rdfs:subClassOf pt:TimePeriod ;
	rdfs:label "Reign"@en ;
	rdfs:comment "The period under a single monarch."@en ;
	rdf:isDefinedBy <http://parliament.uk/ontologies/time-period/> .

pt:ParliamentPeriod rdf:type owl:Class ;
	rdfs:subClassOf pt:TimePeriod ;
	rdfs:label "ParliamentPeriod"@en ;
	rdfs:comment "The period of a single parliament between the state opening of the first session and dissolution. Defined as 5 years since the Fixed Term Parliament Act except in exceptional circumstances. Parliament periods are the same across both houses."@en ;
	rdf:isDefinedBy <http://parliament.uk/ontologies/time-period/> .

pt:DissolutionPeriod rdf:type owl:Class ;
	rdfs:subClassOf pt:TimePeriod ;
	rdfs:label "DissolutionPeriod"@en ;
	rdfs:comment "The period between parliament periods during which Parliament is dissolved and does not exist. During this time there are no members, no committees etc. Dissolution periods are the same across both houses."@en ;
	rdf:isDefinedBy <http://parliament.uk/ontologies/time-period/> .

pt:Session rdf:type owl:Class ;
	rdfs:subClassOf pt:TimePeriod ;
	rdfs:label "Session"@en ;
	rdfs:comment "The period during which Parliament is active between any State Opening and prorogation or dissolution. A session typically lasts for one year though isn't bound by that. Any legislation introduced in a session must be passed in both houses during that session, unless it is carried over. Session periods are the same across both houses."@en ;
	rdf:isDefinedBy <http://parliament.uk/ontologies/time-period/> .
	
pt:PorogationPeriod rdf:type owl:Class ;
	rdfs:subClassOf pt:TimePeriod ;
	rdfs:label "PorogationPeriod"@en ;
	rdfs:comment "The period during which Parliament is inactive between prorogation announcement and State Opening.  During this time there are still members but nearly all Parliamentary business stops. Prorogation periods are the same across both houses."@en ;
	rdf:isDefinedBy <http://parliament.uk/ontologies/time-period/> .
	
pt:Term rdf:type owl:Class ;
	rdfs:subClassOf pt:TimePeriod ;
	rdfs:label "Term"@en ;
	rdfs:comment "The period during which Parliament is active and may be sitting between recess periods. Term periods are not necessarily the same across both houses."@en ;
	rdf:isDefinedBy <http://parliament.uk/ontologies/time-period/> .

pt:Recess rdf:type owl:Class ;
	rdfs:subClassOf pt:TimePeriod ;
	rdfs:label "Recess"@en ;
	rdfs:comment "The period during which Parliament is inactive and does not sit between term periods. Recess periods are not necessarily the same across both houses."@en ;
	rdf:isDefinedBy <http://parliament.uk/ontologies/time-period/> .

pt:SittingDay rdf:type owl:Class ;
	rdfs:subClassOf pt:TimePeriod ;
	rdfs:label "SittingDay"@en ;
	rdfs:comment "A day on which a house is sitting. Sitting days are not the same across both houses."@en ;
	rdf:isDefinedBy <http://parliament.uk/ontologies/time-period/> .

pt:House rdf:type owl:Class ;
	rdfs:subClassOf pt:TimePeriod ;
	rdfs:label "House"@en ;
	rdfs:comment "A parliamentary house e.g. the House of Lords."@en ;
	rdf:isDefinedBy <http://parliament.uk/ontologies/time-period/> .


				
#######  Object properties ##### 

pt:initiatesEvent rdf:type owl:ObjectProperty ;
	rdfs:label "initiatesEvent"@en ;
	rdfs:comment "Relates an agent to an event they initiate."@en ;
	rdfs:domain pt:Agent ;
	rdfs:range pt:Event ;
	rdf:isDefinedBy <http://parliament.uk/ontologies/time-period/> .
	
pt:initiatesTimePeriod rdf:type owl:ObjectProperty ;
	rdfs:label "initiatesTimePeriod"@en ;
	rdfs:comment "Relates an event to a time period it initiates."@en ;
	rdfs:domain pt:Event ;
	rdfs:range pt:TimePeriod ;
	rdf:isDefinedBy <http://parliament.uk/ontologies/time-period/> .
	
pt:containedIn rdf:type owl:ObjectProperty ;
	rdfs:label "containedIn"@en ;
	rdfs:comment "Relates an event to a time period it's contained in."@en ;
	rdfs:domain pt:Event ;
	rdfs:range pt:TimePeriod ;
	rdf:isDefinedBy <http://parliament.uk/ontologies/time-period/> .
	
pt:governingParty rdf:type owl:ObjectProperty ;
	rdfs:label "governingParty"@en ;
	rdfs:comment "Relates a government administration period to the party or parties in power."@en ;
	rdfs:domain pt:GovernmentAdministrationPeriod ;
	rdfs:range pt:Party ;
	rdf:isDefinedBy <http://parliament.uk/ontologies/time-period/> .
	
pt:partOfPremiershipPeriod rdf:type owl:ObjectProperty ;
	rdfs:label "partOfPremiershipPeriod"@en ;
	rdfs:comment "Relates a government administration period to a premiership period. e.g. allows for grouping of 3 Thatcher administrations into one 'premiership'."@en ;
	rdfs:domain pt:GovernmentAdministrationPeriod ;
	rdfs:range pt:PremiershipPeriod ;
	rdf:isDefinedBy <http://parliament.uk/ontologies/time-period/> .
	
pt:hasSession rdf:type owl:ObjectProperty ;
	rdfs:label "hasSession"@en ;
	rdfs:comment "Relates a Parliament period to a session."@en ;
	rdfs:domain pt:ParliamentPeriod ;
	rdfs:range pt:Session ;
	rdf:isDefinedBy <http://parliament.uk/ontologies/time-period/> .
	
pt:hasProrogationPeriod rdf:type owl:ObjectProperty ;
	rdfs:label "hasProrogationPeriod"@en ;
	rdfs:comment "Relates a Parliament period to a prorogation period."@en ;
	rdfs:domain pt:ParliamentPeriod ;
	rdfs:range pt:ProrogationPeriod ;
	rdf:isDefinedBy <http://parliament.uk/ontologies/time-period/> .

pt:hasTerm rdf:type owl:ObjectProperty ;
	rdfs:label "hasTerm"@en ;
	rdfs:comment "Relates a session to a term."@en ;
	rdfs:domain pt:Session ;
	rdfs:range pt:Term ;
	rdf:isDefinedBy <http://parliament.uk/ontologies/time-period/> .
	
pt:hasRecess rdf:type owl:ObjectProperty ;
	rdfs:label "hasRecess"@en ;
	rdfs:comment "Relates a session to a recess."@en ;
	rdfs:domain pt:Session ;
	rdfs:range pt:Recess ;
	rdf:isDefinedBy <http://parliament.uk/ontologies/time-period/> .
	
pt:houseHasTerm rdf:type owl:ObjectProperty ;
	rdfs:label "houseHasTerm"@en ;
	rdfs:comment "Relates a house to a term. Allows for different term periods in different houses."@en ;
	rdfs:domain pt:House ;
	rdfs:range pt:Term ;
	rdf:isDefinedBy <http://parliament.uk/ontologies/time-period/> .

pt:houseHasRecess rdf:type owl:ObjectProperty ;
	rdfs:label "houseHasRecess"@en ;
	rdfs:comment "Relates a house to a recess. Allows for different recess periods in different houses."@en ;
	rdfs:domain pt:House ;
	rdfs:range pt:Recess ;
	rdf:isDefinedBy <http://parliament.uk/ontologies/time-period/> .
	
pt:hasSittingDay rdf:type owl:ObjectProperty ;
	rdfs:label "hasSittingDay"@en ;
	rdfs:comment "Relates a term to a sitting day."@en ;
	rdfs:domain pt:Term ;
	rdfs:range pt:SittingDay ;
	rdf:isDefinedBy <http://parliament.uk/ontologies/time-period/> .
	
pt:recallSittingDay rdf:type owl:ObjectProperty ;
	rdfs:label "recallSittingDay"@en ;
	rdfs:comment "Relates a recess to a sitting day. Allows for sitting days in recess if Parliament is recalled."@en ;
	rdfs:domain pt:Recess ;
	rdfs:range pt:SittingDay ;
	rdf:isDefinedBy <http://parliament.uk/ontologies/time-period/> .
	
	
	
#######  Data properties ##### 

pt:proposedStartDate rdf:type owl:DatatypeProperty ;
	rdfs:label "proposedStartDate"@en ;
	rdfs:comment "Time period has a proposed start date."@en ;
	rdfs:domain pt:TimePeriod ;
	rdfs:range xsd:date ;
	rdf:isDefinedBy <http://parliament.uk/ontologies/time-period/> .
pt:proposedEndDate rdf:type owl:DatatypeProperty ;
	rdfs:label "proposedEndDate"@en ;
	rdfs:comment "Time period has a proposed end date."@en ;
	rdfs:domain pt:TimePeriod ;
	rdfs:range xsd:date ;
	rdf:isDefinedBy <http://parliament.uk/ontologies/time-period/> .
pt:parliamentNumber rdf:type owl:DatatypeProperty ;
	rdfs:label "parliamentNumber"@en ;
	rdfs:comment "Parliament period has an ordinal number. Numbered from the Act of Union 1800."@en ;
	rdfs:domain pt:ParliamentPeriod ;
	rdfs:range xsd:integer ;
	rdf:isDefinedBy <http://parliament.uk/ontologies/time-period/> .